proofs/lean/treehash-equivalence/Treehash.lean
@@ -2,3 +2,4 @@ import Treehash.Basic
 import Treehash.Recursive
 import Treehash.Iter
 import Treehash.Theorems
+import Treehash.Auth
